some bounded pointwise_decision

CM2_UBOUNDED_dec.v
@@ -6,13 +6,60 @@ Require Import M2.CM2 M2.CM2_facts.
 Section Construction.
 Variable M : Cm2.
 
-Notation bounded := (bounded M).
+Notation multi_step := (CM2.multi_step M).
+Notation bounded := (CM2.bounded M).
+
+Definition path k x := map (fun n => if multi_step n x is Some y then y else x) (seq 0 k).
+
+Lemma length_path {k x} : length (path k x) = k.
+Proof. by rewrite /path map_length seq_length. Qed.
+
+Lemma Config_eq_dec (x y : Config) : {x = y} + {x <> y}.
+Proof. by do ? decide equality. Qed.
+
+Lemma pointwise_decision K x : {bounded K x} + {not (bounded K x)}.
+Proof.
+  case HK: (multi_step K x) => [y|].
+  - have [Hy|Hy] := In_dec Config_eq_dec y (path K x).
+    + left. exists (path K x). rewrite length_path.
+      split; first done.
+      move: (Hy) => /in_map_iff [k].
+      case Hk: (multi_step k x) => [z|]; first last.
+      { move=> [_] /in_seq ?.
+        by move: Hk HK => /(multi_step_k_monotone K) /(_ ltac:(lia)) ->. }
+      move=> [?] /in_seq ?. subst z.
+      move=> z [k'].
+      have [?|?] : k' < K \/ K <= k' by lia.
+      { move=> Hk'. apply /in_map_iff. exists k'.
+        rewrite Hk'. split; first done. apply /in_seq. lia. }
+      have -> : k' = k + (k'-k) by lia.
+      rewrite (Nat.div_mod_eq (k'-k) (K-k)).
+      rewrite (multi_step_plus Hk).
+      have := Nat.mod_upper_bound (k' - k) (K - k) ltac:(lia).
+      move: (_ / _) (_ mod _) => n k'' ?.
+      have : multi_step ((K - k) * n) y = Some y.
+      { rewrite (ltac:(lia) : K = k + (K - k)) (multi_step_plus Hk) in HK.
+        move: (K - k) HK => m Hm. elim: n; first by rewrite Nat.mul_0_r.
+        move=> n IH. by rewrite Nat.mul_succ_r Nat.add_comm (multi_step_plus Hm). }
+      move=> /multi_step_plus -> Hk''. apply /in_map_iff. exists (k+k'').
+      rewrite (multi_step_plus Hk) Hk''. split; first done.
+      apply /in_seq. lia.
+    + right. admit.
+  - left. exists (path K x). rewrite length_path. split; first done.
+    move=> y [k]. have [?|?] : k < K \/ K <= k by lia.
+    + move=> Hk. apply /in_map_iff. exists k. rewrite Hk in_seq.
+      split; [done|lia].
+    + by move: HK => /(multi_step_k_monotone k) /(_ ltac:(lia)) ->.
+Admitted.
+
 
 Lemma fixed_decision K : 
   {forall x : Config, bounded K x} + {~ (forall x : Config, bounded K x)}.
 Proof.
   have := Forall_dec (fun 'x => bounded K x) _
     (list_prod (seq 0 (length M)) (list_prod (seq 0 (K+1)) (seq 0 (K+1)))).
+
+
 Admitted.
 
 Lemma uniform_decision : (uniformly_bounded M) + (not (uniformly_bounded M)).
